src/PowerFunc.v
@@ -1,0 +1,44 @@
+
+Section PowerFunc.
+
+  Context {T: Type}.
+
+  Definition power_func(f: T -> T): nat -> (T -> T) :=
+    fix rec(n: nat) := match n with
+    | O => fun x => x
+    | S m => fun x => f ((rec m) x)
+    end.
+
+  Lemma power_func_one_plus_n: forall f n initial,
+    power_func f n (f initial) = f (power_func f n initial).
+  Proof.
+    intros f n. induction n; intros.
+    - reflexivity.
+    - simpl. f_equal. apply IHn.
+  Qed.
+
+  (* TODO probably we won't need multiApply any more *)
+
+  Definition multiApply(f: T -> T)(init: T): nat -> T :=
+    fix rec(n: nat) := match n with
+    | O => init
+    | S m => f (rec m)
+    end.
+
+  Lemma multiApply_is_power_func: forall n f init,
+    multiApply f init n = power_func f n init.
+  Proof.
+    induction n; intros.
+    - reflexivity.
+    - simpl. f_equal. apply IHn.
+  Qed.
+
+  Lemma multiApply_inv: forall (f: T -> T) (init: T) (n: nat),
+    multiApply f init (S n) = multiApply f (f init) n.
+  Proof.
+    intros. simpl. induction n.
+    - reflexivity.
+    - simpl. f_equal. assumption.
+  Qed.
+
+End PowerFunc.
